steel/Zeta.Steel.VerifierTypes.fst
@@ -38,7 +38,7 @@ type thread_state_t = {
   store        : vstore;
   clock        : R.ref U64.t;
   epoch_hashes : AEH.all_epoch_hashes;
-  last_verified_epoch: R.ref M.epoch_id;
+  last_verified_epoch: R.ref (option M.epoch_id);
   processed_entries: G.ref (Seq.seq log_entry);
   app_results  : G.ref M.app_results;
   serialization_buffer: A.larray U8.t 4096
